examples/n_german/nGerman.thy
@@ -28,7 +28,7 @@ definition n_RecvGntE :: "nat \<Rightarrow> rule" where
     assign (Para ''Cache.State'' i, Const E) ||
     assign (Para ''Chan2.Cmd'' i, Const Empty)"
 
-lemma RecvGntE:
+lemma symRecvGntE:
   "symParamRule N n_RecvGntE"
   "wellFormedStatement N (act (n_RecvGntE i))"
   "absTransfRule M (n_RecvGntE i) = (if i \<le> M then n_RecvGntE i else chaos \<triangleright> skip)"
@@ -41,7 +41,7 @@ definition n_RecvGntS :: "nat \<Rightarrow> rule" where
     assign (Para ''Cache.State'' i, Const S) ||
     assign (Para ''Chan2.Cmd'' i, Const Empty)"
 
-lemma RecvGntS:
+lemma symRecvGntS:
   "symParamRule N n_RecvGntS"
   "wellFormedStatement N (act (n_RecvGntS i))"
   "absTransfRule M (n_RecvGntS i) = (if i \<le> M then n_RecvGntS i else chaos \<triangleright> skip)"
@@ -70,7 +70,7 @@ definition n_SendGntE_abs :: "nat \<Rightarrow> rule" where
     assign (Ident ''ExGntd'', Const true) ||
     assign (Ident ''CurCmd'', Const Empty)"
 
-lemma wellFormedSendGntE:
+lemma symSendGntE:
   "symParamRule N (n_SendGntE N)"
   "wellFormedStatement N (act (n_SendGntE N i))"
   unfolding n_SendGntE_def
@@ -101,7 +101,7 @@ definition n_SendGntS_abs :: "nat \<Rightarrow> rule" where
    \<triangleright>
     assign (Ident ''CurCmd'', Const Empty)"
 
-lemma wellFormedSendGntS:
+lemma symSendGntS:
   "symParamRule N n_SendGntS"
   "wellFormedStatement N (act (n_SendGntS i))"
   unfolding n_SendGntS_def
@@ -129,7 +129,7 @@ definition n_RecvInvAck1_abs :: rule where
    \<triangleright>
     assign (Ident ''ExGntd'', Const false)"
 
-lemma RecvInvAck1:
+lemma symRecvInvAck1:
   "symParamRule N n_RecvInvAck1"
   "wellFormedStatement N (act (n_RecvInvAck1 i))"
   "absTransfRule M (n_RecvInvAck1 i) = (if i \<le> M then n_RecvInvAck1 i else n_RecvInvAck1_abs)"
@@ -151,7 +151,7 @@ definition n_RecvInvAck2_abs :: rule where
    \<triangleright>
     skip"
 
-lemma RecvInvAck2:
+lemma symRecvInvAck2:
   "symParamRule N n_RecvInvAck2"
   "wellFormedStatement N (act (n_RecvInvAck2 i))"
   "absTransfRule M (n_RecvInvAck2 i) = (if i \<le> M then n_RecvInvAck2 i else n_RecvInvAck2_abs)"
@@ -167,7 +167,7 @@ definition n_SendInvAck1 :: "nat \<Rightarrow> rule" where
     assign (Para ''Chan3.Cmd'' i, Const InvAck) ||
     assign (Para ''Cache.State'' i, Const I)"
 
-lemma SendInvAck1:
+lemma symSendInvAck1:
   "symParamRule N n_SendInvAck1"
   "wellFormedStatement N (act (n_SendInvAck1 i))"
   "absTransfRule M (n_SendInvAck1 i) = (if i \<le> M then n_SendInvAck1 i else chaos \<triangleright> skip)"
@@ -183,7 +183,7 @@ definition n_SendInvAck2 :: "nat \<Rightarrow> rule" where
     assign (Para ''Chan3.Cmd'' i, Const InvAck) ||
     assign (Para ''Cache.State'' i, Const I)"
 
-lemma SendInvAck2:
+lemma symSendInvAck2:
   "symParamRule N n_SendInvAck2"
   "wellFormedStatement N (act (n_SendInvAck2 i))"
   "absTransfRule M (n_SendInvAck2 i) = (if i \<le> M then n_SendInvAck2 i else chaos \<triangleright> skip)"
@@ -204,7 +204,7 @@ definition n_SendInv1_abs :: rule where
    \<triangleright>
     skip"
 
-lemma SendInv1:
+lemma symSendInv1:
   "symParamRule N n_SendInv1"
   "wellFormedStatement N (act (n_SendInv1 i))"
   "absTransfRule M (n_SendInv1 i) = (if i \<le> M then n_SendInv1 i else n_SendInv1_abs)"
@@ -227,7 +227,7 @@ definition n_SendInv2_abs :: rule where
    \<triangleright>
     skip"
 
-lemma SendInv2:
+lemma symSendInv2:
   "symParamRule N n_SendInv2"
   "wellFormedStatement N (act (n_SendInv2 i))"
   "absTransfRule M (n_SendInv2 i) = (if i \<le> M then n_SendInv2 i else n_SendInv2_abs)"
@@ -251,7 +251,7 @@ definition n_RecvReqE_abs :: "nat \<Rightarrow> rule" where
     assign (Ident ''CurPtr'', Const (index (M+1))) ||
     forallStm (\<lambda>j. assign (Para ''InvSet'' j, IVar (Para ''ShrSet'' j))) M"
 
-lemma wellFormedReqE:
+lemma symRecvReqE:
   "symParamRule N (n_RecvReqE N)"
   "wellFormedStatement N (act (n_RecvReqE N i))"
   unfolding n_RecvReqE_def
@@ -280,7 +280,7 @@ definition n_RecvReqS_abs :: "nat \<Rightarrow> rule" where
     assign (Ident ''CurPtr'', Const (index (M+1))) ||
     forallStm (\<lambda>j. assign (Para ''InvSet'' j, IVar (Para ''ShrSet'' j))) M"
 
-lemma wellFormedRecvReqS:
+lemma symRecvReqS:
   "symParamRule N (n_RecvReqS N)"
   "wellFormedStatement N (act (n_RecvReqS N i))"
   unfolding n_RecvReqS_def
@@ -299,7 +299,7 @@ definition n_SendReqE1 :: "nat \<Rightarrow> rule" where
    \<triangleright>
     assign (Para ''Chan1.Cmd'' i, Const ReqE)"
 
-lemma SendReqE1:
+lemma symSendReqE1:
   "symParamRule N n_SendReqE1"
   "wellFormedStatement N (act (n_SendReqE1 i))"
   "absTransfRule M (n_SendReqE1 i) = (if i \<le> M then n_SendReqE1 i else chaos \<triangleright> skip)"
@@ -312,7 +312,7 @@ definition n_SendReqE2 :: "nat \<Rightarrow> rule" where
    \<triangleright>
     assign (Para ''Chan1.Cmd'' i, Const ReqE)"
 
-lemma SendReqE2:
+lemma symSendReqE2:
   "symParamRule N n_SendReqE2"
   "wellFormedStatement N (act (n_SendReqE2 i))"
   "absTransfRule M (n_SendReqE2 i) = (if i \<le> M then n_SendReqE2 i else chaos \<triangleright> skip)"
@@ -349,6 +349,135 @@ definition rules :: "nat \<Rightarrow> rule set" where
     (\<exists>i. i\<le>N \<and> r=n_SendReqE2 i) \<or>
     (\<exists>i. i\<le>N \<and> r=n_SendReqS i)
   }"
+definition n_RecvGntEs::" nat\<Rightarrow>rule set" where [simp]:
+  "n_RecvGntEs N== oneParamCons N  n_RecvGntE"
+
+definition n_RecvGntSs::" nat\<Rightarrow>rule set" where [simp]:
+  "n_RecvGntSs N== oneParamCons N  n_RecvGntS"
+
+definition n_SendGntEs::" nat\<Rightarrow>rule set" where [simp]:
+  "n_SendGntEs N== oneParamCons N  (n_SendGntE N)"
+
+definition n_SendGntSs::" nat\<Rightarrow>rule set" where [simp]:
+  "n_SendGntSs N== oneParamCons N  n_SendGntS"
+
+definition n_RecvInvAck1s::" nat\<Rightarrow>rule set" where [simp]:
+  "n_RecvInvAck1s N== oneParamCons N  n_RecvInvAck1"
+
+definition n_RecvInvAck2s::" nat\<Rightarrow>rule set" where [simp]:
+  "n_RecvInvAck2s N== oneParamCons N  n_RecvInvAck2"
+
+definition n_SendInvAck1s::" nat\<Rightarrow>rule set" where [simp]:
+  "n_SendInvAck1s N== oneParamCons N  (n_SendInvAck1 )"
+
+definition n_SendInvAck2s::" nat\<Rightarrow>rule set" where [simp]:
+  "n_SendInvAck2s N== oneParamCons N  (n_SendInvAck2 )"
+
+definition n_SendInv1s::" nat\<Rightarrow>rule set" where [simp]:
+  "n_SendInv1s N== oneParamCons N n_SendInv1"
+
+definition n_SendInv2s::" nat\<Rightarrow>rule set" where [simp]:
+  "n_SendInv2s N== oneParamCons N  (n_SendInv2 )"
+
+definition n_RecvReqEs::" nat\<Rightarrow>rule set" where [simp]:
+  "n_RecvReqEs N== oneParamCons N  (n_RecvReqE N )"
+
+definition n_RecvReqSs::" nat\<Rightarrow>rule set" where [simp]:
+  "n_RecvReqSs N== oneParamCons N (n_RecvReqS N)"
+
+definition n_SendReqE1s::" nat\<Rightarrow>rule set" where [simp]:
+  "n_SendReqE1s N== oneParamCons N n_SendReqE1"
+
+definition n_SendReqE2s::" nat\<Rightarrow>rule set" where [simp]:
+  "n_SendReqE2s N== oneParamCons N  n_SendReqE2 "
+
+definition n_SendReqSs::" nat\<Rightarrow>rule set" where [simp]:
+  "n_SendReqSs N== oneParamCons N  (n_SendReqS )"
+
+ 
+definition rules' :: "nat \<Rightarrow> rule set" where [simp]:
+  "rules' N \<equiv>  (n_RecvGntEs N) \<union>
+    (n_RecvGntSs N) \<union>
+    (n_SendGntEs  N) \<union>
+    (n_SendGntSs N) \<union>
+    ( n_RecvInvAck1s N)\<union>
+    ( n_RecvInvAck2s N) \<union>
+    ( n_SendInvAck1s N) \<union>
+    ( n_SendInvAck2s N) \<union>
+    ( n_SendInv1s N) \<union>
+    ( n_SendInv2s N) \<union>
+    ( n_RecvReqEs  N) \<union>
+    ( n_RecvReqSs  N) \<union>
+    ( n_SendReqE1s N) \<union>
+    ( n_SendReqE2s N) \<union>
+    ( n_SendReqSs N)  
+   "
+lemma n_RecvGntEsIsSym:
+  "symProtRules' N (n_RecvGntEs N)"
+  using symRecvGntE(1) n_RecvGntEs_def symParaRuleInfSymRuleSet by auto
+
+lemma n_RecvGntSsIsSym:
+  "symProtRules' N (n_RecvGntSs N)"
+  using n_RecvGntSs_def symRecvGntS(1) symParaRuleInfSymRuleSet by auto 
+
+lemma n_SendGntEsIsSym:
+  "symProtRules' N (n_SendGntEs N)"
+  using n_SendGntEs_def symSendGntE(1) symParaRuleInfSymRuleSet by auto 
+
+lemma n_SendGntSsIsSym:
+  "symProtRules' N (n_SendGntSs N)"  
+  using n_SendGntSs_def symSendGntS(1) symParaRuleInfSymRuleSet by auto
+
+lemma  n_RecvInvAck1sIsSym:
+  "symProtRules' N ( n_RecvInvAck1s N)"
+  using symRecvInvAck1(1)  n_RecvInvAck1s_def symParaRuleInfSymRuleSet by auto
+
+lemma n_RecvInvAck2sIsSym:
+  "symProtRules' N (n_RecvInvAck2s N)"
+  using n_RecvInvAck2s_def symRecvInvAck2(1) symParaRuleInfSymRuleSet by auto 
+
+lemma n_SendInvAck1sIsSym:
+  "symProtRules' N (n_SendInvAck1s N)"
+  using n_SendInvAck1s_def symSendInvAck1(1) symParaRuleInfSymRuleSet by auto 
+
+lemma n_SendInvAck2sIsSym:
+  "symProtRules' N (n_SendInvAck2s N)"
+  using n_SendInvAck2s_def symSendInvAck2(1) symParaRuleInfSymRuleSet by auto 
+
+lemma n_SendInv1sIsSym:
+  "symProtRules' N (n_SendInv1s N)"
+  using n_SendInv1s_def symSendInv1(1) symParaRuleInfSymRuleSet by auto 
+
+lemma n_SendInv2sIsSym:
+  "symProtRules' N (n_SendInv2s N)"
+  using n_SendInv2s_def symSendInv2(1) symParaRuleInfSymRuleSet by auto 
+
+lemma n_RecvReqEsIsSym:
+  "symProtRules' N (n_RecvReqEs N)"
+  using n_RecvReqEs_def symRecvReqE(1) symParaRuleInfSymRuleSet by auto 
+
+lemma n_RecvReqSsIsSym:
+  "symProtRules' N (n_RecvReqSs N)"
+  using n_RecvReqSs_def symRecvReqS(1) symParaRuleInfSymRuleSet by auto 
+
+lemma n_SendReqE1sIsSym:
+  "symProtRules' N (n_SendReqE1s N)"
+  using n_SendReqE1s_def symSendReqE1(1) symParaRuleInfSymRuleSet by auto 
+
+lemma n_SendReqE2sIsSym:
+  "symProtRules' N (n_SendReqE2s N)"
+  using n_SendReqE2s_def symSendReqE2(1) symParaRuleInfSymRuleSet by auto 
+
+lemma n_SendReqSsIsSym:
+  "symProtRules' N (n_SendReqSs N)"
+  using n_SendReqSs_def symSendReqS(1) symParaRuleInfSymRuleSet by auto
+ 
+
+lemma rulesSym':
+  shows "symProtRules' N (rules' N)"
+  using n_RecvGntEsIsSym n_RecvGntSsIsSym n_RecvInvAck1sIsSym n_RecvInvAck2sIsSym n_RecvReqEsIsSym n_RecvReqSsIsSym n_SendGntEsIsSym n_SendGntSsIsSym n_SendInv1sIsSym n_SendInv2sIsSym n_SendInvAck1sIsSym n_SendInvAck2sIsSym n_SendReqE1sIsSym 
+n_SendReqE2sIsSym n_SendReqSsIsSym rules'_def symProtRulesUnion by presburger 
+ 
 
 definition initSpec0 :: "nat \<Rightarrow> formula" where
   "initSpec0 N \<equiv> (\<forall>\<^sub>fi. IVar (Para ''Chan1.Cmd'' i) =\<^sub>f Const Empty) N"
@@ -405,9 +534,14 @@ definition invAux :: "nat \<Rightarrow> nat \<Rightarrow> formula" where
      IVar (Para ''Chan3.Cmd'' i) =\<^sub>f Const InvAck \<and>\<^sub>f
      \<not>\<^sub>f IVar (Ident ''CurCmd'') =\<^sub>f Const Empty \<and>\<^sub>f
      IVar (Ident ''ExGntd'') =\<^sub>f Const true \<longrightarrow>\<^sub>f
-     forallFormExcl (\<lambda>j. \<not>\<^sub>f IVar (Para ''Cache.State'' j) =\<^sub>f Const E) i N \<and>\<^sub>f
+    forallFormExcl 
+    (\<lambda>j. ((\<not>\<^sub>f (IVar (Para ''Cache.State'' j) =\<^sub>f Const E))  \<and>\<^sub>f
+       ( \<not>\<^sub>f (IVar (Para ''Chan2.Cmd'' j) =\<^sub>f Const GntE))  \<and>\<^sub>f
+       ( \<not>\<^sub>f (IVar (Para ''Chan3.Cmd'' j) =\<^sub>f Const InvAck))
+    )) i N"
+     (*forallFormExcl (\<lambda>j. \<not>\<^sub>f IVar (Para ''Cache.State'' j) =\<^sub>f Const E) i N \<and>\<^sub>f
      forallFormExcl (\<lambda>j. \<not>\<^sub>f IVar (Para ''Chan2.Cmd'' j) =\<^sub>f Const GntE) i N \<and>\<^sub>f
-     forallFormExcl (\<lambda>j. \<not>\<^sub>f IVar (Para ''Chan3.Cmd'' j) =\<^sub>f Const InvAck) i N"
+     forallFormExcl (\<lambda>j. \<not>\<^sub>f IVar (Para ''Chan3.Cmd'' j) =\<^sub>f Const InvAck) i N"*)
 
 definition n_RecvInvAck1' :: "nat \<Rightarrow> nat \<Rightarrow> rule" where
   "n_RecvInvAck1' N i = strengthenRule2 (invAux N i) (n_RecvInvAck1 i)"
@@ -417,9 +551,11 @@ definition n_RecvInvAck1'_ref :: "nat \<Rightarrow> nat \<Rightarrow> rule" wher
     (IVar (Para ''Chan3.Cmd'' i) =\<^sub>f Const InvAck \<and>\<^sub>f
      \<not>\<^sub>f IVar (Ident ''CurCmd'') =\<^sub>f Const Empty \<and>\<^sub>f
      IVar (Ident ''ExGntd'') =\<^sub>f Const true) \<and>\<^sub>f
-    forallFormExcl (\<lambda>j. \<not>\<^sub>f IVar (Para ''Cache.State'' j) =\<^sub>f Const E) i N \<and>\<^sub>f
-    forallFormExcl (\<lambda>j. \<not>\<^sub>f IVar (Para ''Chan2.Cmd'' j) =\<^sub>f Const GntE) i N \<and>\<^sub>f
-    forallFormExcl (\<lambda>j. \<not>\<^sub>f IVar (Para ''Chan3.Cmd'' j) =\<^sub>f Const InvAck) i N
+   forallFormExcl 
+    (\<lambda>j. ((\<not>\<^sub>f (IVar (Para ''Cache.State'' j) =\<^sub>f Const E))  \<and>\<^sub>f
+       ( \<not>\<^sub>f (IVar (Para ''Chan2.Cmd'' j) =\<^sub>f Const GntE))  \<and>\<^sub>f
+       ( \<not>\<^sub>f (IVar (Para ''Chan3.Cmd'' j) =\<^sub>f Const InvAck))
+    )) i N
    \<triangleright>
     assign (Para ''Chan3.Cmd'' i, Const Empty) ||
     assign (Para ''ShrSet'' i, Const false) ||
@@ -429,9 +565,10 @@ definition n_RecvInvAck1'_abs :: "nat \<Rightarrow> rule" where
   "n_RecvInvAck1'_abs M \<equiv>
     (\<not>\<^sub>f IVar (Ident ''CurCmd'') =\<^sub>f Const Empty \<and>\<^sub>f
      IVar (Ident ''ExGntd'') =\<^sub>f Const true) \<and>\<^sub>f
-    forallForm (\<lambda>j. \<not>\<^sub>f IVar (Para ''Cache.State'' j) =\<^sub>f Const E) M \<and>\<^sub>f
-    forallForm (\<lambda>j. \<not>\<^sub>f IVar (Para ''Chan2.Cmd'' j) =\<^sub>f Const GntE) M \<and>\<^sub>f
-    forallForm (\<lambda>j. \<not>\<^sub>f IVar (Para ''Chan3.Cmd'' j) =\<^sub>f Const InvAck) M
+    forallForm(\<lambda>j. ((\<not>\<^sub>f (IVar (Para ''Cache.State'' j) =\<^sub>f Const E))  \<and>\<^sub>f
+       ( \<not>\<^sub>f (IVar (Para ''Chan2.Cmd'' j) =\<^sub>f Const GntE))  \<and>\<^sub>f
+       ( \<not>\<^sub>f (IVar (Para ''Chan3.Cmd'' j) =\<^sub>f Const InvAck))
+    )) M  
    \<triangleright>
     assign (Ident ''ExGntd'', Const false)"
 
@@ -450,5 +587,43 @@ lemma absRecvInvAck1'b:
   "M \<le> N \<Longrightarrow> absTransfRule M (n_RecvInvAck1'_ref N i) =
     (if i \<le> M then n_RecvInvAck1 i else n_RecvInvAck1'_abs M)"
   unfolding n_RecvInvAck1_def n_RecvInvAck1'_ref_def n_RecvInvAck1'_abs_def by auto
+
+
+definition pair1:: "((nat\<Rightarrow>formula)\<times>(nat\<Rightarrow>formula))" where [simp]:
+ "pair1 ==(%i. IVar (Para ''Chan3.Cmd'' i) =\<^sub>f Const InvAck \<and>\<^sub>f
+     \<not>\<^sub>f IVar (Ident ''CurCmd'') =\<^sub>f Const Empty \<and>\<^sub>f
+     IVar (Ident ''ExGntd'') =\<^sub>f Const true  ,
+                  (\<lambda>j. ((\<not>\<^sub>f (IVar (Para ''Cache.State'' j) =\<^sub>f Const E))  \<and>\<^sub>f
+       ( \<not>\<^sub>f (IVar (Para ''Chan2.Cmd'' j) =\<^sub>f Const GntE))  \<and>\<^sub>f
+       ( \<not>\<^sub>f (IVar (Para ''Chan3.Cmd'' j) =\<^sub>f Const InvAck))))
+    ) "
+
+definition F::"((nat\<Rightarrow>formula)\<times>(nat\<Rightarrow>formula)) set" where [simp]:
+"F \<equiv> {pair1}"
+
+  
+definition n_RecvInvAck12s::" nat \<Rightarrow>rule set" where [simp]:
+  "n_RecvInvAck12s N==
+  (oneParamCons N  (%i. (strengthenRule2  (constrInvByExcl pair1 i N) (n_RecvInvAck1 i))))"
+
+  
+definition rules2' :: "nat \<Rightarrow> rule set" where [simp]:
+  "rules2' N \<equiv>  (n_RecvGntEs N) \<union>
+    (n_RecvGntSs N) \<union>
+    (n_SendGntEs  N) \<union>
+    (n_SendGntSs N) \<union>
+    ( n_RecvInvAck12s N)\<union>
+    ( n_RecvInvAck2s N) \<union>
+    ( n_SendInvAck1s N) \<union>
+    ( n_SendInvAck2s N) \<union>
+    ( n_SendInv1s N) \<union>
+    ( n_SendInv2s N) \<union>
+    ( n_RecvReqEs  N) \<union>
+    ( n_RecvReqSs  N) \<union>
+    ( n_SendReqE1s N) \<union>
+    ( n_SendReqE2s N) \<union>
+    ( n_SendReqSs N)  
+    "
+
 
 end
